

$$f[x_1, x_0] = \frac{f(x_1) - f(x_0)}{x_1 - x_0}$$

$$f[x_2, x_1, x_0] = \frac{f[x_2, x_1] - f[x_1, x_0]}{x_2 - x_0}$$

$$f(x_i, x_j, x_n) = \frac{f[x_i, x_j] - f[x_j, x_n]}{x_i - x_n}$$

### Ejercicio

x	f(x)
0	1
1	0
4	1.386294
5	1.609438
6	1.791752

Calcular  $f(2)$  usando interpolación lineal, cuadrática y cúbica

✓ Lineal

$$f_1(x) = \frac{f(x_1) - f(x_0)}{x_1 - x_0} (x - x_0) + f(x_0)$$

$$f_1(2) = \frac{1.386294 - 0}{4 - 1} (2 - 1) + 0$$

$$f_1(2) = 0.462098$$

### Cuadrática

$$f_2(x) = b_0 + b_1(x - x_0) + b_2(x - x_0)(x - x_1)$$

$$b_0 = f(x_0) = 0$$

$$b_1 = \frac{f(x_1) - f(x_0)}{x_1 - x_0} = \frac{1.386294 - 0}{4 - 1} = 0.462098$$

$$b_2 = \frac{f(x_2) - f(x_1)}{x_2 - x_1} - \frac{f(x_1) - f(x_0)}{x_1 - x_0} = \frac{1.609438 - 1.386294}{5 - 4} - \frac{1.386294 - 0}{4 - 1}$$

$$b_2 = \frac{0.223144}{1} - 0.462098 = -0.0597385$$

$$f_2(x) = 0 + 0.462098(2 - 1) + (-0.0597385)(2 - 1)(2 - 4)$$

$$f_2(2) = 0 + 0.462098 + 0.119477 = 0.581575$$

Cubica

$$f_3(x) = b_0 + b_1(x-x_0) + b_2(x-x_0)(x-x_1) + b_3(x-x_0)(x-x_1)(x-x_2)$$

$$f_3(x_2) = f(x_0) + \frac{f(x_1) - f(x_0)}{x_1 - x_0} (x_2 - x_0) + \left( \frac{f(x_2) - f(x_1)}{x_2 - x_1} - \frac{f(x_1) - f(x_0)}{x_1 - x_0} \right) (x_2 - x_0)(x_2 - x_1)$$

$$+ b_3 (x - x_0)(x - x_1)(x - x_2)$$

$$b_3 =$$

Polinomio de interpolación de Newton

$$f[x_n, x_{n-1}, x_1, x_0] = \frac{f[x_n, x_{n-1}, x_1] - f[x_n, x_{n-1}, x_2, x_0]}{x_n - x_0}$$

$$f[x_3, x_2, x_1, x_0] = \frac{f[x_3, x_2, x_1] - f[x_3, x_2, x_0]}{x_3 - x_0}$$

$$= \frac{f[x_3, x_2, x_1] - f[x_3, x_2, x_0]}{x_3 - x_0} = \frac{f[x_3, x_2, x_1] - f[x_3, x_2, x_0]}{x_3 - x_0}$$

$$f[x_3, x_2, x_1, x_0] = \frac{f(x_3, x_2, x_1) - f(x_3, x_2, x_0)}{x_3 - x_0}$$

$$= \frac{f(x_3, x_2) - f(x_2, x_1)}{x_3 - x_1} - \frac{f(x_3, x_2) - f(x_2, x_0)}{x_3 - x_0}$$

$$= \frac{f(x_3) - f(x_2)}{x_3 - x_1} - \frac{f(x_3) - f(x_1)}{x_3 - x_1} - \frac{f(x_3) - f(x_2)}{x_3 - x_0} - \frac{f(x_1) - f(x_0)}{x_3 - x_0}$$

$$= \frac{f(x_3) - f(x_2)}{x_3 - x_1} - \frac{f(x_3) - f(x_1)}{x_3 - x_1} - \frac{f(x_3) - f(x_2)}{x_3 - x_0}$$

$$= \frac{f(x_3) - f(x_2)}{x_3 - x_1} - \frac{f(x_2) - f(x_1)}{x_3 - x_1} - \frac{f(x_3) - f(x_2)}{x_3 - x_0} - \frac{f(x_2) - f(x_0)}{x_3 - x_0} = b_3$$

$$= \frac{1.797752 - 1.609438}{6 - 4} - \frac{1.609438 - 1.386204}{6 - 4} - \frac{1.797752 - 1.609438}{6 - 1} - \frac{1.609438 - 0}{6 - 1}$$

$$= \frac{0.091157 - 0.111572 - 0.0364628 - 0.3218876}{5} = -0.07575308$$

$$f_3(2) = 0 + 0.462098(1) + (-0.0597385)(2-1)(2-4) + (-0.07575308)(1)(2-4)(2-5)$$

$$= 0 + 0.462098 + 0.119477 - 0.45451848$$

$$\underline{f_3(2) = 0.12705652}$$